tuned names

thys/Gale_Shapley/Gale_Shapley1.thy
@@ -68,12 +68,12 @@ type_synonym prefs = "nat list list"
 
 locale Pref =
 fixes n
-fixes P\<^sub>a :: prefs
-fixes P\<^sub>b :: prefs
-defines "n \<equiv> length P\<^sub>a"
-assumes length_P\<^sub>b: "length P\<^sub>b = n"
-assumes P\<^sub>a_set: "a < n  \<Longrightarrow> length(P\<^sub>a!a) = n \<and> set(P\<^sub>a!a) = {<n}"
-assumes P\<^sub>b_set: "b < n \<Longrightarrow> length(P\<^sub>b!b) = n \<and> set(P\<^sub>b!b) = {<n}"
+fixes P :: prefs
+fixes Q :: prefs
+defines "n \<equiv> length P"
+assumes length_Q: "length Q = n"
+assumes P_set: "a < n  \<Longrightarrow> length(P!a) = n \<and> set(P!a) = {<n}"
+assumes Q_set: "b < n \<Longrightarrow> length(Q!b) = n \<and> set(Q!b) = {<n}"
 begin
 
 
@@ -148,21 +148,21 @@ proof -
   finally show ?thesis .
 qed
 
-definition "match A a = P\<^sub>a ! a ! (A ! a)"
+definition "match A a = P ! a ! (A ! a)"
 
 lemma match_less_n: "\<lbrakk> wf A; a < n \<rbrakk> \<Longrightarrow> match A a < n"
-by (metis P\<^sub>a_set atLeastLessThan_iff match_def nth_mem subset_eq)
+by (metis P_set atLeastLessThan_iff match_def nth_mem subset_eq)
 
 lemma match_upd_neq: "\<lbrakk> wf A; a < n; a \<noteq> a' \<rbrakk> \<Longrightarrow> match (A[a := b]) a' = match A a'"
 by (simp add: match_def)
 
 definition stable :: "nat list \<Rightarrow> nat set \<Rightarrow> bool" where
-"stable A M = (\<not>(\<exists>a\<in>M. \<exists>a'\<in>M. P\<^sub>a ! a \<turnstile> match A a' < match A a \<and> P\<^sub>b ! match A a' \<turnstile> a < a'))"
+"stable A M = (\<not>(\<exists>a\<in>M. \<exists>a'\<in>M. P ! a \<turnstile> match A a' < match A a \<and> Q ! match A a' \<turnstile> a < a'))"
 
 text \<open>The set of Bs that an A would prefer to its current match,
 i.e. all Bs above its current match \<open>A!a\<close>.\<close>
 abbreviation preferred where
-"preferred A a == nth (P\<^sub>a!a) ` {<A!a}"
+"preferred A a == nth (P!a) ` {<A!a}"
 
 definition matching where [simp]:
 "matching A M = (wf A \<and> inj_on (match A) M)"
@@ -176,9 +176,9 @@ and a: "a < n \<and> a \<notin> M" and final: "A ! a + 1 = n"
 shows "insert a M = {<n}"
 proof -
   let ?B = "preferred A a"
-  have "(!) (P\<^sub>a ! a) ` {<n} = {<n}" by (metis P\<^sub>a_set a map_nth set_map set_upt)
-  hence "inj_on ((!) (P\<^sub>a ! a)) {<n}" by(simp add: eq_card_imp_inj_on)
-  hence "inj_on ((!) (P\<^sub>a ! a)) {<A!a}" using final by(simp add: subset_inj_on)
+  have "(!) (P ! a) ` {<n} = {<n}" by (metis P_set a map_nth set_map set_upt)
+  hence "inj_on ((!) (P ! a)) {<n}" by(simp add: eq_card_imp_inj_on)
+  hence "inj_on ((!) (P ! a)) {<A!a}" using final by(simp add: subset_inj_on)
   hence 1: "Suc(card ?B) = n" using final by (simp add: card_image)
   have 2: "card ?B \<le> card M"
     by(rule surj_card_le[OF subset_eq_atLeast0_lessThan_finite[OF M] pref_match'])
@@ -197,10 +197,10 @@ proof (rule ccontr)
   assume "\<not> A ! a + 1 < n"
   hence "A ! a + 1 = n" using A \<open>a < n\<close> unfolding matching_def
     by (metis add.commute wf_less_n linorder_neqE_nat not_less_eq plus_1_eq_Suc)
-  hence *: "nth (P\<^sub>a ! a) ` {<n} \<subseteq> match A ` M"
+  hence *: "nth (P ! a) ` {<n} \<subseteq> match A ` M"
     using pref_match' matched less_Suc_eq match_def by fastforce
-  have "nth (P\<^sub>a!a) ` {<n} = {<n}"
-    using P\<^sub>a_set[OF  \<open>a < n\<close>] by (metis map_nth set_map set_upt)
+  have "nth (P!a) ` {<n} = {<n}"
+    using P_set[OF  \<open>a < n\<close>] by (metis map_nth set_map set_upt)
   hence "{<n} \<subseteq> match A ` M" using * by metis
   hence "card {<n} \<le> card M"
     using finite_subset[OF \<open>M \<subseteq> {<n}\<close> finite_atLeastLessThan] by (metis surj_card_le)
@@ -298,60 +298,60 @@ if \<open>a\<close> prefers \<open>b\<close> over \<open>a\<close>'s current mat
 then \<open>b\<close> is matched with an \<open>a'\<close> that \<open>b\<close> prefers to \<open>a\<close>.\<close>
 
 definition pref_match where
-"pref_match A M = (\<forall>a<n. \<forall>b<n. P\<^sub>a!a \<turnstile> b < match A a \<longrightarrow> (\<exists>a'\<in>M. b = match A a' \<and> P\<^sub>b ! b \<turnstile> a' < a))"
+"pref_match A M = (\<forall>a<n. \<forall>b<n. P!a \<turnstile> b < match A a \<longrightarrow> (\<exists>a'\<in>M. b = match A a' \<and> Q ! b \<turnstile> a' < a))"
 
 definition pref_match' where
-"pref_match' A M = (\<forall>a<n. \<forall>b \<in> preferred A a. \<exists>a'\<in>M. b = match A a' \<and> P\<^sub>b ! b \<turnstile> a' < a)"
+"pref_match' A M = (\<forall>a<n. \<forall>b \<in> preferred A a. \<exists>a'\<in>M. b = match A a' \<and> Q ! b \<turnstile> a' < a)"
 
 lemma pref_match'_iff: "wf A \<Longrightarrow> pref_match' A M = pref_match A M"
 apply (auto simp add: pref_match'_def pref_match_def imp_ex prefers_def match_def)
-  apply (smt (verit) P\<^sub>a_set atLeast0LessThan order.strict_trans index_first lessThan_iff linorder_neqE_nat nth_index)
-  by (smt (verit, best) P\<^sub>a_set atLeast0LessThan card_atLeastLessThan card_distinct diff_zero in_mono index_nth_id lessThan_iff less_trans nth_mem)
+  apply (smt (verit) P_set atLeast0LessThan order.strict_trans index_first lessThan_iff linorder_neqE_nat nth_index)
+  by (smt (verit, best) P_set atLeast0LessThan card_atLeastLessThan card_distinct diff_zero in_mono index_nth_id lessThan_iff less_trans nth_mem)
 
 definition opti\<^sub>a where
 "opti\<^sub>a A = (\<nexists>A'. matching A' {<n} \<and> stable A' {<n} \<and>
-                (\<exists>a<n. P\<^sub>a ! a \<turnstile> match A' a < match A a))"
+                (\<exists>a<n. P ! a \<turnstile> match A' a < match A a))"
 
 definition pessi\<^sub>b where
 "pessi\<^sub>b A = (\<nexists>A'. matching A' {<n} \<and> stable A' {<n} \<and>
-                 (\<exists>a<n. \<exists>a'<n. match A a = match A' a' \<and> P\<^sub>b ! match A a \<turnstile> a < a'))"
+                 (\<exists>a<n. \<exists>a'<n. match A a = match A' a' \<and> Q ! match A a \<turnstile> a < a'))"
 
 lemma opti\<^sub>a_pessi\<^sub>b: assumes "opti\<^sub>a A" shows "pessi\<^sub>b A"
 unfolding pessi\<^sub>b_def
 proof (safe, goal_cases)
   case (1 A' a a')
-  have "\<not> P\<^sub>a!a \<turnstile>  match A a <  match A' a" using 1
+  have "\<not> P!a \<turnstile>  match A a <  match A' a" using 1
     by (metis atLeast0LessThan lessThan_iff stable_def)
-  with 1 \<open>opti\<^sub>a A\<close> show ?case using P\<^sub>a_set match_less_n opti\<^sub>a_def prefers_def unfolding matching_def
+  with 1 \<open>opti\<^sub>a A\<close> show ?case using P_set match_less_n opti\<^sub>a_def prefers_def unfolding matching_def
     by (metis (no_types) atLeast0LessThan inj_on_contraD lessThan_iff less_not_refl linorder_neqE_nat nth_index)
 qed
 
 lemma opti\<^sub>a_inv:
 assumes A: "wf A" and a: "a < n" and a': "a' < n" and same_match: "match A a' = match A a"
-and pref: "P\<^sub>b ! match A a' \<turnstile> a' < a" and "opti\<^sub>a A"
+and pref: "Q ! match A a' \<turnstile> a' < a" and "opti\<^sub>a A"
 shows "opti\<^sub>a (A[a := A ! a + 1])"
 proof (unfold opti\<^sub>a_def matching_def, rule notI, elim exE conjE)
   note opti\<^sub>a = \<open>opti\<^sub>a A\<close>[unfolded opti\<^sub>a_def matching_def]
   let ?A = "A[a := A ! a + 1]"
   fix A' a''
   assume "a'' < n" and A': "length A' = n" "set A' \<subseteq> {<n}" "stable A' {<n}" "inj_on (match A') {<n}"
-  and pref_a'': "P\<^sub>a ! a'' \<turnstile> match A' a'' < match ?A a''"
+  and pref_a'': "P ! a'' \<turnstile> match A' a'' < match ?A a''"
   show False
   proof cases
     assume [simp]: "a'' = a"
     have "A!a < n" using A a by(simp add: subset_eq)
-    with A A' a pref_a'' have "P\<^sub>a ! a \<turnstile> match A' a < match A a \<or> match A' a = match A a"
+    with A A' a pref_a'' have "P ! a \<turnstile> match A' a < match A a \<or> match A' a = match A a"
       apply(auto simp: prefers_def match_def)
-      by (smt (verit) P\<^sub>a_set wf_less_n card_atLeastLessThan card_distinct diff_zero index_nth_id
+      by (smt (verit) P_set wf_less_n card_atLeastLessThan card_distinct diff_zero index_nth_id
               not_less_eq not_less_less_Suc_eq)
     thus False
     proof
-      assume "P\<^sub>a ! a \<turnstile> match A' a < match A a " thus False using opti\<^sub>a A' \<open>a < n\<close> by(fastforce) 
+      assume "P ! a \<turnstile> match A' a < match A a " thus False using opti\<^sub>a A' \<open>a < n\<close> by(fastforce) 
     next
       assume "match A' a = match A a"
       have "a \<noteq> a'" using pref a' by(auto simp: prefers_def)
-      hence "P\<^sub>a ! a' \<turnstile> match A' a < match A' a' \<and> P\<^sub>b ! match A' a \<turnstile> a' < a" using opti\<^sub>a pref A' same_match \<open>match A' a = match A a\<close> a a'
-        by (metis P\<^sub>a_set atLeast0LessThan match_less_n inj_onD lessThan_iff linorder_neqE_nat nth_index prefers_def)
+      hence "P ! a' \<turnstile> match A' a < match A' a' \<and> Q ! match A' a \<turnstile> a' < a" using opti\<^sub>a pref A' same_match \<open>match A' a = match A a\<close> a a'
+        by (metis P_set atLeast0LessThan match_less_n inj_onD lessThan_iff linorder_neqE_nat nth_index prefers_def)
       thus False using a a' \<open>a \<noteq> a'\<close> A'(3) by (metis stable_def atLeastLessThan_iff zero_le)
     qed
   next
@@ -376,7 +376,7 @@ by(simp add: pref_match_def)
 
 lemma invAM_swap:
 assumes "invAM A M"
-assumes a: "a < n \<and> a \<notin> M" and a': "a' \<in> M \<and> match A a' = match A a" and pref: "P\<^sub>b ! match A a' \<turnstile> a < a'"
+assumes a: "a < n \<and> a \<notin> M" and a': "a' \<in> M \<and> match A a' = match A a" and pref: "Q ! match A a' \<turnstile> a < a'"
 shows "invAM (A[a' := A!a'+1]) (M - {a'} \<union> {a})"
 proof -
   have A: "wf A" and M : "M \<subseteq> {<n}" and inj: "inj_on (match A) M" and pref_match: "pref_match A M"
@@ -412,14 +412,14 @@ qed
 
 lemma invAM_next:
 assumes "invAM A M"
-assumes a: "a < n \<and> a \<notin> M" and a': "a' \<in> M \<and> match A a' = match A a" and pref: "\<not> P\<^sub>b ! match A a' \<turnstile> a < a'"
+assumes a: "a < n \<and> a \<notin> M" and a': "a' \<in> M \<and> match A a' = match A a" and pref: "\<not> Q ! match A a' \<turnstile> a < a'"
 shows "invAM (A[a := A!a + 1]) M"
 proof -
   have A: "wf A" and M : "M \<subseteq> {<n}" and inj: "inj_on (match A) M" and pref_match: "pref_match A M"
   and opti\<^sub>a: "opti\<^sub>a A" and "a' < n"
     by(insert \<open>invAM A M\<close> a') (auto)
-  hence pref': "P\<^sub>b ! match A a' \<turnstile> a' < a"
-    using pref a a' P\<^sub>b_set unfolding prefers_def
+  hence pref': "Q ! match A a' \<turnstile> a' < a"
+    using pref a a' Q_set unfolding prefers_def
     by (metis match_def match_less_n index_eq_index_conv linorder_less_linear subsetD)
   have "M \<noteq> {<n}" using a by fastforce
   have neq_a: "\<forall>x. x\<in> M \<longrightarrow> a \<noteq> x" using a by blast
@@ -448,7 +448,7 @@ lemma Gale_Shapley1: "VARS M A a a' b
   IF b \<notin> match A ` M
   THEN M := M \<union> {a}
   ELSE a' := (SOME a'. a' \<in> M \<and> match A a' = b);
-       IF P\<^sub>b ! match A a' \<turnstile> a < a'
+       IF Q ! match A a' \<turnstile> a < a'
        THEN A[a'] := A!a'+1; M := M - {a'} \<union> {a}
        ELSE A[a] := A!a+1
        FI
@@ -457,7 +457,7 @@ lemma Gale_Shapley1: "VARS M A a a' b
  [matching A {<n} \<and> stable A {<n} \<and> opti\<^sub>a A]"
 proof (vcg_tc, goal_cases)
   case 1 thus ?case
-   by(auto simp: stable_def opti\<^sub>a_def pref_match_def P\<^sub>a_set card_distinct match_def index_nth_id prefers_def)
+   by(auto simp: stable_def opti\<^sub>a_def pref_match_def P_set card_distinct match_def index_nth_id prefers_def)
 next
   case 3 thus ?case using pref_match_stable by auto
 next
@@ -535,7 +535,7 @@ lemma Gale_Shapley2: "VARS A a a' as b
   IF b \<notin> match A ` ({<n} - set as)
   THEN as := tl as
   ELSE a' := (SOME a'. a' \<in> {<n} - set as \<and> match A a' = b);
-       IF P\<^sub>b ! match A a' \<turnstile> a < a'
+       IF Q ! match A a' \<turnstile> a < a'
        THEN A[a'] := A!a'+1; as := a' # tl as
        ELSE A[a] := A!a+1
        FI
@@ -544,7 +544,7 @@ lemma Gale_Shapley2: "VARS A a a' as b
  [matching A {<n} \<and> stable A {<n} \<and> opti\<^sub>a A]"
 proof (vcg_tc, goal_cases)
   case 1 thus ?case
-   by(auto simp: stable_def opti\<^sub>a_def pref_match_def P\<^sub>a_set card_distinct match_def index_nth_id prefers_def)
+   by(auto simp: stable_def opti\<^sub>a_def pref_match_def P_set card_distinct match_def index_nth_id prefers_def)
 next
   case 3 thus ?case using pref_match_stable by auto
 next
@@ -634,7 +634,7 @@ lemma Gale_Shapley3: "VARS A B a a' as b
   IF B b = None
   THEN B := B(b := Some a); as := tl as
   ELSE a' := the(B b);
-       IF P\<^sub>b ! match A a' \<turnstile> a < a'
+       IF Q ! match A a' \<turnstile> a < a'
        THEN B := B(b := Some a); A[a'] := A!a'+1; as := a' # tl as
        ELSE A[a] := A!a+1
        FI
@@ -643,7 +643,7 @@ lemma Gale_Shapley3: "VARS A B a a' as b
  [matching A {<n} \<and> stable A {<n} \<and> opti\<^sub>a A]"
 proof (vcg_tc, goal_cases)
   case 1 thus ?case
-    by(auto simp: stable_def opti\<^sub>a_def pref_match_def P\<^sub>a_set card_distinct match_def index_nth_id prefers_def)
+    by(auto simp: stable_def opti\<^sub>a_def pref_match_def P_set card_distinct match_def index_nth_id prefers_def)
 next
   case 3 thus ?case using pref_match_stable by auto
 next
@@ -739,7 +739,7 @@ lemma Gale_Shapley4_unused: "VARS A B M a a' as b
   IF \<not> (M ! b)
   THEN M[b] := True; B[b] := a; as := tl as
   ELSE a' := B ! b;
-       IF P\<^sub>b ! match A a' \<turnstile> a < a'
+       IF Q ! match A a' \<turnstile> a < a'
        THEN B[b] := a; A[a'] := A!a'+1; as := a' # tl as
        ELSE A[a] := A!a+1
        FI
@@ -748,7 +748,7 @@ lemma Gale_Shapley4_unused: "VARS A B M a a' as b
  [wf A \<and> inj_on (match A) {<n} \<and> stable A {<n} \<and> opti\<^sub>a A]"
 proof (vcg_tc, goal_cases)
   case 1 thus ?case
-   by(auto simp: stable_def opti\<^sub>a_def pref_match_def P\<^sub>a_set card_distinct match_def index_nth_id prefers_def)
+   by(auto simp: stable_def opti\<^sub>a_def pref_match_def P_set card_distinct match_def index_nth_id prefers_def)
 next
   case 3 thus ?case using pref_match_stable by auto
 next
@@ -853,7 +853,7 @@ lemma Gale_Shapley4:
   INV { invAM A ({<ai+1} - {a}) \<and> invAB A B ({<ai+1} - {a}) \<and> (a \<le> ai \<and> ai < n) \<and> z = n-ai }
   VAR {var A {<ai}}
   DO a' := the(B (match A a));
-     IF P\<^sub>b ! match A a' \<turnstile> a < a'
+     IF Q ! match A a' \<turnstile> a < a'
      THEN B := B(match A a := Some a); A[a'] := A!a'+1; a := a'
      ELSE A[a] := A!a+1
      FI
@@ -863,7 +863,7 @@ lemma Gale_Shapley4:
  [matching A {<n} \<and> stable A {<n} \<and> opti\<^sub>a A]"
 proof (vcg_tc, goal_cases)
   case 1 thus ?case  (* outer invar holds initially *)
-   by(auto simp: stable_def pref_match_def P\<^sub>a_set card_distinct match_def index_nth_id prefers_def opti\<^sub>a_def)[]
+   by(auto simp: stable_def pref_match_def P_set card_distinct match_def index_nth_id prefers_def opti\<^sub>a_def)[]
 next
   case 2 (* outer invar and b implies inner invar *)
   thus ?case by (auto simp: atLeastLessThanSuc_atLeastAtMost simp flip: atLeastLessThan_eq_atLeastAtMost_diff)
@@ -983,7 +983,7 @@ lemma Gale_Shapley4_var2:
   INV { invAM A ({<ai+1} - {a}) \<and> invAB A B ({<ai+1} - {a}) \<and> (a \<le> ai \<and> ai < n) \<and> z = n-ai }
   VAR {var2 A}
   DO a' := the(B (match A a));
-     IF P\<^sub>b ! match A a' \<turnstile> a < a'
+     IF Q ! match A a' \<turnstile> a < a'
      THEN B := B(match A a := Some a); A[a'] := A!a'+1; a := a'
      ELSE A[a] := A!a+1
      FI
@@ -993,7 +993,7 @@ lemma Gale_Shapley4_var2:
  [matching A {<n} \<and> stable A {<n} \<and> opti\<^sub>a A]"
 proof (vcg_tc, goal_cases)
   case 1 thus ?case  (* outer invar holds initially *)
-   by(auto simp: stable_def pref_match_def P\<^sub>a_set card_distinct match_def index_nth_id prefers_def opti\<^sub>a_def)[]
+   by(auto simp: stable_def pref_match_def P_set card_distinct match_def index_nth_id prefers_def opti\<^sub>a_def)[]
 next
   case 2 (* outer invar and b implies inner invar *)
   thus ?case by (auto simp: atLeastLessThanSuc_atLeastAtMost simp flip: atLeastLessThan_eq_atLeastAtMost_diff)
@@ -1074,7 +1074,7 @@ lemma Gale_Shapley4_1: "VARS A B a a' ai b
   IF B b = None
   THEN B := B(b := Some a); ai := ai + 1; a := ai
   ELSE a' := the(B b);
-       IF P\<^sub>b ! match A a' \<turnstile> a < a'
+       IF Q ! match A a' \<turnstile> a < a'
        THEN B := B(b := Some a); A[a'] := A!a'+1; a := a'
        ELSE A[a] := A!a+1
        FI
@@ -1083,7 +1083,7 @@ lemma Gale_Shapley4_1: "VARS A B a a' ai b
  [matching A {<n} \<and> stable A {<n} \<and> opti\<^sub>a A]"
 proof (vcg_tc, goal_cases)
   case 1 thus ?case
-    by(auto simp: stable_def opti\<^sub>a_def pref_match_def P\<^sub>a_set card_distinct match_def index_nth_id prefers_def)
+    by(auto simp: stable_def opti\<^sub>a_def pref_match_def P_set card_distinct match_def index_nth_id prefers_def)
 next
   case 3 thus ?case using pref_match_stable
     using atLeast0_lessThan_Suc by force
@@ -1194,7 +1194,7 @@ lemma Gale_Shapley5:
   INV { invar2 A B M ai a \<and> z = n-ai }
   VAR {var A {<ai}}
   DO a' := B ! match A a;
-     IF P\<^sub>b ! match A a' \<turnstile> a < a'
+     IF Q ! match A a' \<turnstile> a < a'
      THEN B[match A a] := a; A[a'] := A!a'+1; a := a'
      ELSE A[a] := A!a+1
      FI
@@ -1204,7 +1204,7 @@ lemma Gale_Shapley5:
  [matching A {<n} \<and> stable A {<n} \<and> opti\<^sub>a A]"
 proof (vcg_tc, goal_cases)
   case 1 thus ?case  (* outer invar holds initially *)
-   by(auto simp: pref_match_def P\<^sub>a_set card_distinct match_def index_nth_id prefers_def opti\<^sub>a_def \<alpha>_def cong: conj_cong)
+   by(auto simp: pref_match_def P_set card_distinct match_def index_nth_id prefers_def opti\<^sub>a_def \<alpha>_def cong: conj_cong)
 next
   case 2 (* outer invar and b implies inner invar *)
   thus ?case by (auto simp: atLeastLessThanSuc_atLeastAtMost simp flip: atLeastLessThan_eq_atLeastAtMost_diff)
@@ -1286,7 +1286,7 @@ lemma Gale_Shapley5_var2:
   INV { invar2 A B M ai a \<and> z = n-ai }
   VAR {var2 A}
   DO a' := B ! match A a;
-     IF P\<^sub>b ! match A a' \<turnstile> a < a'
+     IF Q ! match A a' \<turnstile> a < a'
      THEN B[match A a] := a; A[a'] := A!a'+1; a := a'
      ELSE A[a] := A!a+1
      FI
@@ -1296,7 +1296,7 @@ lemma Gale_Shapley5_var2:
  [matching A {<n} \<and> stable A {<n} \<and> opti\<^sub>a A]"
 proof (vcg_tc, goal_cases)
   case 1 thus ?case  (* outer invar holds initially *)
-   by(auto simp: pref_match_def P\<^sub>a_set card_distinct match_def index_nth_id prefers_def opti\<^sub>a_def \<alpha>_def cong: conj_cong)
+   by(auto simp: pref_match_def P_set card_distinct match_def index_nth_id prefers_def opti\<^sub>a_def \<alpha>_def cong: conj_cong)
 next
   case 2 (* outer invar and b implies inner invar *)
   thus ?case by (auto simp: atLeastLessThanSuc_atLeastAtMost simp flip: atLeastLessThan_eq_atLeastAtMost_diff)
@@ -1377,8 +1377,8 @@ shows
   "(\<not> M ! b \<longrightarrow>
     invar2' A (B[b := a]) (M[b := True]) (ai + 1) (ai + 1) \<and> var A ({<ai + 1 + 1} - {ai + 1}) < v) \<and>
    (M ! b \<longrightarrow>
-    (P\<^sub>b ! match A a' \<turnstile> a < a' \<longrightarrow> invar2' A1 (B[b := a]) M ai a' \<and> var A1 ({<ai + 1} - {a'}) < v) \<and>
-    (\<not> P\<^sub>b ! match A a' \<turnstile> a < a' \<longrightarrow> invar2' A2 B M ai a \<and> var A2 ({<ai + 1} - {a}) < v))"
+    (Q ! match A a' \<turnstile> a < a' \<longrightarrow> invar2' A1 (B[b := a]) M ai a' \<and> var A1 ({<ai + 1} - {a'}) < v) \<and>
+    (\<not> Q ! match A a' \<turnstile> a < a' \<longrightarrow> invar2' A2 B M ai a \<and> var A2 ({<ai + 1} - {a}) < v))"
 proof -
   let ?M = "{<ai+1} - {a}"
   have invAM: "invAM A ?M" and m: "matching A ?M" and A: "wf A" and M: "?M \<subseteq> {<n}"
@@ -1457,7 +1457,7 @@ lemma Gale_Shapley5_1: "VARS A B M a a' ai b
   IF \<not> M ! b
   THEN B[b] := a; M[b] := True; ai := ai + 1; a := ai
   ELSE a' := B ! b;
-       IF P\<^sub>b ! match A a' \<turnstile> a < a'
+       IF Q ! match A a' \<turnstile> a < a'
        THEN B[b] := a; A[a'] := A!a'+1; a := a'
        ELSE A[a] := A!a+1
        FI
@@ -1466,7 +1466,7 @@ lemma Gale_Shapley5_1: "VARS A B M a a' ai b
  [matching A {<n} \<and> stable A {<n} \<and> opti\<^sub>a A]"
 proof (vcg_tc, goal_cases)
   case 1 thus ?case
-   by(auto simp: pref_match_def P\<^sub>a_set card_distinct match_def index_nth_id prefers_def opti\<^sub>a_def \<alpha>_def cong: conj_cong)
+   by(auto simp: pref_match_def P_set card_distinct match_def index_nth_id prefers_def opti\<^sub>a_def \<alpha>_def cong: conj_cong)
 next
   case 3 thus ?case using pref_match_stable
     using atLeast0_lessThan_Suc by force
@@ -1477,7 +1477,7 @@ next
 qed
 
 
-subsection \<open>Algorithm 6: replace \<open>P\<^sub>b\<close> by ranking \<open>R\<^sub>b\<close>\<close>
+subsection \<open>Algorithm 6: replace \<open>Q\<close> by ranking \<open>R\<close>\<close>
 
 lemma inner_to_outer:
 assumes inv: "invar2 A B M ai a \<and> b = match A a" and not_b: "\<not> M ! b"
@@ -1495,7 +1495,7 @@ proof -
 qed
 
 lemma inner_pres:
-assumes R: "\<forall>b<n. \<forall>a1<n. \<forall>a2<n. R ! b ! a1 < R ! b ! a2 \<longleftrightarrow> P\<^sub>b ! b \<turnstile> a1 < a2" and
+assumes R: "\<forall>b<n. \<forall>a1<n. \<forall>a2<n. R ! b ! a1 < R ! b ! a2 \<longleftrightarrow> Q ! b \<turnstile> a1 < a2" and
   inv: "invar2 A B M ai a" and m: "M ! b" and v: "var A {<ai} = v"
   and after: "A1 = A[a' := A ! a' + 1]" "A2 = A[a := A ! a + 1]"
     "a' = B!b" "r = R ! match A a'" "b = match A a"
@@ -1518,8 +1518,8 @@ proof -
   proof ((rule;rule;rule), goal_cases)
     have *: "{<ai + 1} - {a} - {?a} \<union> {a} = {<ai + 1} - {?a}" using inv a' by auto
     case 1
-    hence unstab: "P\<^sub>b ! match A a' \<turnstile> a < a'"
-      using R a a' as P\<^sub>b_set P\<^sub>a_set match_less_n[OF A] n_def length_P\<^sub>b R by (simp)
+    hence unstab: "Q ! match A a' \<turnstile> a < a'"
+      using R a a' as Q_set P_set match_less_n[OF A] n_def length_Q R by (simp)
     have inj_dom: "inj_on (\<alpha> B M) (dom (\<alpha> B M))" by (metis (mono_tags) domD inj_onI invAB)
     have invAB': "invAB A1 (\<alpha> (B[match A a := a]) M) ({<ai + 1} - {?a})"
       using invAB_swap[OF invAB a a' inj_dom] * match_less_n[OF A] a m
@@ -1533,8 +1533,8 @@ proof -
   next
     have *: "\<forall>b. b < n \<and> M!b \<longrightarrow> a \<noteq> B!b" by (metis invAB ranI \<alpha>_Some a)
     case 3
-    hence unstab: "\<not> P\<^sub>b ! match A a' \<turnstile> a < a'"
-      using R a a' as P\<^sub>b_set P\<^sub>a_set match_less_n[OF A] n_def length_P\<^sub>b
+    hence unstab: "\<not> Q ! match A a' \<turnstile> a < a'"
+      using R a a' as Q_set P_set match_less_n[OF A] n_def length_Q
       by (simp add: ranking_iff_pref)
     then show ?case using invAM_next[OF invAM a a'] 3 inv * by (simp add: match_def)
   next
@@ -1547,7 +1547,7 @@ qed
 text \<open>First, the `old' version with the more complicated inner variant:\<close>
 
 lemma Gale_Shapley6:
-assumes "R\<^sub>b = map ranking P\<^sub>b"
+assumes "R = map ranking Q"
 shows
 "VARS A B M ai a a' b r
  [ai = 0 \<and> A = replicate n 0 \<and> length B = n \<and> M = replicate n False]
@@ -1558,7 +1558,7 @@ shows
   WHILE M ! b
   INV { invar2 A B M ai a \<and> b = match A a \<and> z = n-ai }
   VAR {var A {<ai}}
-  DO a' := B ! b; r := R\<^sub>b ! match A a';
+  DO a' := B ! b; r := R ! match A a';
      IF r ! a < r ! a'
      THEN B[b] := a; A[a'] := A!a'+1; a := a'
      ELSE A[a] := A!a+1
@@ -1570,14 +1570,14 @@ shows
  [matching A {<n} \<and> stable A {<n} \<and> opti\<^sub>a A]"
 proof (vcg_tc, goal_cases)
   case 1 thus ?case  (* outer invar holds initially *)
-   by(auto simp: stable_def pref_match_def P\<^sub>a_set card_distinct match_def index_nth_id prefers_def opti\<^sub>a_def \<alpha>_def cong: conj_cong)
+   by(auto simp: stable_def pref_match_def P_set card_distinct match_def index_nth_id prefers_def opti\<^sub>a_def \<alpha>_def cong: conj_cong)
 next
   case 2 (* outer invar and b implies inner invar *)
   thus ?case by (auto simp: atLeastLessThanSuc_atLeastAtMost simp flip: atLeastLessThan_eq_atLeastAtMost_diff)
 next
   case 3 (* preservation of inner invar *)
-  have R: "\<forall>b<n. \<forall>a1<n. \<forall>a2<n. R\<^sub>b ! b ! a1 < R\<^sub>b ! b ! a2 \<longleftrightarrow> P\<^sub>b ! b \<turnstile> a1 < a2"
-    by (simp add: P\<^sub>b_set \<open>R\<^sub>b = _\<close> length_P\<^sub>b ranking_iff_pref)
+  have R: "\<forall>b<n. \<forall>a1<n. \<forall>a2<n. R ! b ! a1 < R ! b ! a2 \<longleftrightarrow> Q ! b \<turnstile> a1 < a2"
+    by (simp add: Q_set \<open>R = _\<close> length_Q ranking_iff_pref)
   show ?case
   proof (simp only: mem_Collect_eq prod.case, goal_cases)
     case 1 show ?case using inner_pres[OF R _ _ refl refl refl] 3 by blast
@@ -1596,7 +1596,7 @@ next
 qed
 
 lemma inner_pres_var2:
-assumes R: "\<forall>b<n. \<forall>a1<n. \<forall>a2<n. R ! b ! a1 < R ! b ! a2 \<longleftrightarrow> P\<^sub>b ! b \<turnstile> a1 < a2" and
+assumes R: "\<forall>b<n. \<forall>a1<n. \<forall>a2<n. R ! b ! a1 < R ! b ! a2 \<longleftrightarrow> Q ! b \<turnstile> a1 < a2" and
   inv: "invar2 A B M ai a" and m: "M ! b" and v: "var2 A = v"
   and after: "A1 = A[a' := A ! a' + 1]" "A2 = A[a := A ! a + 1]"
     "a' = B!b" "r = R ! match A a'" "b = match A a"
@@ -1619,8 +1619,8 @@ proof -
     have *: "{<ai + 1} - {a} - {?a} \<union> {a} = {<ai + 1} - {?a}" using inv a' by auto
     note invAM' =  invAM_swap[OF invAM a a']
     case 1
-    hence unstab: "P\<^sub>b ! match A a' \<turnstile> a < a'"
-      using R a a' as P\<^sub>b_set P\<^sub>a_set match_less_n[OF A] n_def length_P\<^sub>b R by (simp)
+    hence unstab: "Q ! match A a' \<turnstile> a < a'"
+      using R a a' as Q_set P_set match_less_n[OF A] n_def length_Q R by (simp)
     have inj_dom: "inj_on (\<alpha> B M) (dom (\<alpha> B M))" by (metis (mono_tags) domD inj_onI invAB)
     have invAB': "invAB A1 (\<alpha> (B[match A a := a]) M) ({<ai + 1} - {?a})"
       using invAB_swap[OF invAB a a' inj_dom] * match_less_n[OF A] a m
@@ -1634,8 +1634,8 @@ proof -
     have *: "\<forall>b. b < n \<and> M!b \<longrightarrow> a \<noteq> B!b" by (metis invAB ranI \<alpha>_Some a)
     note invAM' = invAM_next[OF invAM a a']
     case 3
-    hence unstab: "\<not> P\<^sub>b ! match A a' \<turnstile> a < a'"
-      using R a a' as P\<^sub>b_set P\<^sub>a_set match_less_n[OF A] n_def length_P\<^sub>b
+    hence unstab: "\<not> Q ! match A a' \<turnstile> a < a'"
+      using R a a' as Q_set P_set match_less_n[OF A] n_def length_Q
       by (simp add: ranking_iff_pref)
     then show ?case using invAM' 3 inv * by (simp add: match_def)
 
@@ -1647,7 +1647,7 @@ qed
 text \<open>The definitive version with variant @{const var2}:\<close>
 
 lemma Gale_Shapley6_var2:
-assumes "R\<^sub>b = map ranking P\<^sub>b"
+assumes "R = map ranking Q"
 shows
 "VARS A B M ai a a' b r
  [ai = 0 \<and> A = replicate n 0 \<and> length B = n \<and> M = replicate n False]
@@ -1658,7 +1658,7 @@ shows
   WHILE M ! b
   INV { invar2 A B M ai a \<and> b = match A a \<and> z = n-ai }
   VAR {var2 A}
-  DO a' := B ! b; r := R\<^sub>b ! match A a';
+  DO a' := B ! b; r := R ! match A a';
      IF r ! a < r ! a'
      THEN B[b] := a; A[a'] := A!a'+1; a := a'
      ELSE A[a] := A!a+1
@@ -1670,14 +1670,14 @@ shows
  [matching A {<n} \<and> stable A {<n} \<and> opti\<^sub>a A]"
 proof (vcg_tc, goal_cases)
   case 1 thus ?case  (* outer invar holds initially *)
-   by(auto simp: stable_def pref_match_def P\<^sub>a_set card_distinct match_def index_nth_id prefers_def opti\<^sub>a_def \<alpha>_def cong: conj_cong)
+   by(auto simp: stable_def pref_match_def P_set card_distinct match_def index_nth_id prefers_def opti\<^sub>a_def \<alpha>_def cong: conj_cong)
 next
   case 2 (* outer invar and b implies inner invar *)
   thus ?case by (auto simp: atLeastLessThanSuc_atLeastAtMost simp flip: atLeastLessThan_eq_atLeastAtMost_diff)
 next
   case 3 (* preservation of inner invar *)
-  have R: "\<forall>b<n. \<forall>a1<n. \<forall>a2<n. R\<^sub>b ! b ! a1 < R\<^sub>b ! b ! a2 \<longleftrightarrow> P\<^sub>b ! b \<turnstile> a1 < a2"
-    by (simp add: P\<^sub>b_set \<open>R\<^sub>b = _\<close> length_P\<^sub>b ranking_iff_pref)
+  have R: "\<forall>b<n. \<forall>a1<n. \<forall>a2<n. R ! b ! a1 < R ! b ! a2 \<longleftrightarrow> Q ! b \<turnstile> a1 < a2"
+    by (simp add: Q_set \<open>R = _\<close> length_Q ranking_iff_pref)
   show ?case
   proof (simp only: mem_Collect_eq prod.case, goal_cases)
     case 1 show ?case using inner_pres_var2[OF R _ _ refl refl refl] 3 by blast
@@ -1715,10 +1715,10 @@ qed
 
 
 lemma inner_pres2:
-assumes R: "\<forall>b<n. \<forall>a1<n. \<forall>a2<n. R\<^sub>b ! b ! a1 < R\<^sub>b ! b ! a2 \<longleftrightarrow> P\<^sub>b ! b \<turnstile> a1 < a2" and
+assumes R: "\<forall>b<n. \<forall>a1<n. \<forall>a2<n. R ! b ! a1 < R ! b ! a2 \<longleftrightarrow> Q ! b \<turnstile> a1 < a2" and
   inv: "invar2 A B M ai a" and m: "M ! b" and v: "var0 A {<n} = v"
   and after: "A1 = A[a' := A ! a' + 1]" "A2 = A[a := A ! a + 1]"
-    "a' = B!b" "r = R\<^sub>b ! match A a'" "b = match A a"
+    "a' = B!b" "r = R ! match A a'" "b = match A a"
 shows "(r ! a < r ! a' \<longrightarrow> invar2 A1 (B[b:=a]) M ai a' \<and> var0 A1 {<n} < v) \<and>
   (\<not> r ! a < r ! a' \<longrightarrow> invar2 A2 B M ai a \<and> var0 A2 {<n} < v)"
 proof -
@@ -1739,8 +1739,8 @@ proof -
   proof ((rule;rule;rule), goal_cases)
     have *: "{<ai + 1} - {a} - {?a} \<union> {a} = {<ai + 1} - {?a}" using inv a' by auto
     case 1
-    hence unstab: "P\<^sub>b ! match A a' \<turnstile> a < a'"
-      using R a a' as P\<^sub>b_set P\<^sub>a_set match_less_n[OF A] n_def length_P\<^sub>b R by (simp)
+    hence unstab: "Q ! match A a' \<turnstile> a < a'"
+      using R a a' as Q_set P_set match_less_n[OF A] n_def length_Q R by (simp)
     have inj_dom: "inj_on (\<alpha> B M) (dom (\<alpha> B M))" by (metis (mono_tags) domD inj_onI invAB)
     have invAB': "invAB A1 (\<alpha> (B[match A a := a]) M) ({<ai + 1} - {?a})"
       using invAB_swap[OF invAB a a' inj_dom] * match_less_n[OF A] a m
@@ -1749,21 +1749,21 @@ proof -
       unfolding * by (simp add: insert_absorb \<alpha>update2)
   next
     case 2
-    hence unstab: "P\<^sub>b ! match A a' \<turnstile> a < a'"
-      using R a a' as P\<^sub>b_set P\<^sub>a_set match_less_n[OF A] n_def length_P\<^sub>b R by (simp)
+    hence unstab: "Q ! match A a' \<turnstile> a < a'"
+      using R a a' as Q_set P_set match_less_n[OF A] n_def length_Q R by (simp)
     from invAM_swap[OF invAM a a'] unstab have wf: "wf (A[a' := A ! a' + 1])" by auto
     show ?case using v var0_next2[OF wf] using \<open>B ! match A a < n\<close> assms(5,7,9) by blast
   next
     have *: "\<forall>b. b < n \<and> M!b \<longrightarrow> a \<noteq> B!b" by (metis invAB ranI \<alpha>_Some a)
     case 3
-    hence unstab: "\<not> P\<^sub>b ! match A a' \<turnstile> a < a'"
-      using R a a' as P\<^sub>b_set P\<^sub>a_set match_less_n[OF A] n_def length_P\<^sub>b
+    hence unstab: "\<not> Q ! match A a' \<turnstile> a < a'"
+      using R a a' as Q_set P_set match_less_n[OF A] n_def length_Q
       by (simp add: ranking_iff_pref)
     then show ?case using invAM_next[OF invAM a a'] 3 inv * by (simp add: match_def)
   next
     case 4
-    hence unstab: "\<not> P\<^sub>b ! match A a' \<turnstile> a < a'"
-      using R a a' as P\<^sub>b_set P\<^sub>a_set match_less_n[OF A] n_def length_P\<^sub>b
+    hence unstab: "\<not> Q ! match A a' \<turnstile> a < a'"
+      using R a a' as Q_set P_set match_less_n[OF A] n_def length_Q
       by (simp add: ranking_iff_pref)
     from invAM_next[OF invAM a a'] unstab have wf: "wf (A[a := A ! a + 1])" by auto
     show ?case using v var0_next2[OF wf] a using assms(6) by presburger
@@ -1771,7 +1771,7 @@ proof -
 qed
 
 lemma Gale_Shapley6':
-assumes "R\<^sub>b = map ranking P\<^sub>b"
+assumes "R = map ranking Q"
 shows
 "VARS A B M ai a a' b r
  [ai = 0 \<and> A = replicate n 0 \<and> length B = n \<and> M = replicate n False]
@@ -1782,7 +1782,7 @@ shows
   WHILE M ! b
   INV { invar2 A B M ai a \<and> b = match A a \<and> z = n-ai }
   VAR {var0 A {<n}}
-  DO a' := B ! b; r := R\<^sub>b ! match A a';
+  DO a' := B ! b; r := R ! match A a';
      IF r ! a < r ! a'
      THEN B[b] := a; A[a'] := A!a'+1; a := a'
      ELSE A[a] := A!a+1
@@ -1794,14 +1794,14 @@ shows
  [matching A {<n} \<and> stable A {<n} \<and> opti\<^sub>a A]"
 proof (vcg_tc, goal_cases)
   case 1 thus ?case  (* outer invar holds initially *)
-   by(auto simp: stable_def pref_match_def P\<^sub>a_set card_distinct match_def index_nth_id prefers_def opti\<^sub>a_def \<alpha>_def cong: conj_cong)
+   by(auto simp: stable_def pref_match_def P_set card_distinct match_def index_nth_id prefers_def opti\<^sub>a_def \<alpha>_def cong: conj_cong)
 next
   case 2 (* outer invar and b implies inner invar *)
   thus ?case by (auto simp: atLeastLessThanSuc_atLeastAtMost simp flip: atLeastLessThan_eq_atLeastAtMost_diff)
 next
   case 3 (* preservation of inner invar *)
-  have R: "\<forall>b<n. \<forall>a1<n. \<forall>a2<n. R\<^sub>b ! b ! a1 < R\<^sub>b ! b ! a2 \<longleftrightarrow> P\<^sub>b ! b \<turnstile> a1 < a2"
-    by (simp add: P\<^sub>b_set \<open>R\<^sub>b = _\<close> length_P\<^sub>b ranking_iff_pref)
+  have R: "\<forall>b<n. \<forall>a1<n. \<forall>a2<n. R ! b ! a1 < R ! b ! a2 \<longleftrightarrow> Q ! b \<turnstile> a1 < a2"
+    by (simp add: Q_set \<open>R = _\<close> length_Q ranking_iff_pref)
   show ?case
   proof (simp only: mem_Collect_eq prod.case, goal_cases)
     case 1 show ?case using inner_pres2[OF R _ _ refl refl refl] 3 by blast
@@ -1823,12 +1823,12 @@ qed
 subsubsection \<open>Algorithm 6.1: single-loop variant\<close>
 
 lemma R_iff_P:
-assumes "R\<^sub>b = map ranking P\<^sub>b" "invar2' A B M ai a" "ai < n" "M ! match A a"
-shows "(R\<^sub>b ! match A (B ! match A a) ! a < R\<^sub>b ! match A (B ! match A a) ! (B ! match A a)) =
-  (P\<^sub>b ! match A (B ! match A a) \<turnstile> a < B ! match A a)"
+assumes "R = map ranking Q" "invar2' A B M ai a" "ai < n" "M ! match A a"
+shows "(R ! match A (B ! match A a) ! a < R ! match A (B ! match A a) ! (B ! match A a)) =
+  (Q ! match A (B ! match A a) \<turnstile> a < B ! match A a)"
 proof -
-  have R: "\<forall>b<n. \<forall>a1<n. \<forall>a2<n. R\<^sub>b ! b ! a1 < R\<^sub>b ! b ! a2 \<longleftrightarrow> P\<^sub>b ! b \<turnstile> a1 < a2"
-    by (simp add: P\<^sub>b_set \<open>R\<^sub>b = _\<close> length_P\<^sub>b ranking_iff_pref)
+  have R: "\<forall>b<n. \<forall>a1<n. \<forall>a2<n. R ! b ! a1 < R ! b ! a2 \<longleftrightarrow> Q ! b \<turnstile> a1 < a2"
+    by (simp add: Q_set \<open>R = _\<close> length_Q ranking_iff_pref)
   let ?M = "{<ai+1} - {a}"
   have A: "wf A" and M: "?M \<subseteq> {<n}" and as: "a < n" and invAB: "invAB2 A B M ?M"
       using assms(2,3) by auto
@@ -1840,7 +1840,7 @@ qed
 
 
 lemma Gale_Shapley6_1:
-assumes "R\<^sub>b = map ranking P\<^sub>b"
+assumes "R = map ranking Q"
 shows "VARS A B M a a' ai b r
  [ai = 0 \<and> a = 0 \<and> A = replicate n 0 \<and> length B = n \<and> M = replicate n False]
  WHILE ai < n
@@ -1849,7 +1849,7 @@ shows "VARS A B M a a' ai b r
  DO b := match A a;
   IF \<not> M ! b
   THEN B[b] := a; M[b] := True; ai := ai + 1; a := ai
-  ELSE a' := B ! b; r := R\<^sub>b ! match A a';
+  ELSE a' := B ! b; r := R ! match A a';
        IF r ! a < r ! a'
        THEN B[b] := a; A[a'] := A!a'+1; a := a'
        ELSE A[a] := A!a+1
@@ -1859,14 +1859,14 @@ shows "VARS A B M a a' ai b r
  [matching A {<n} \<and> stable A {<n} \<and> opti\<^sub>a A]"
 proof (vcg_tc, goal_cases)
   case 1 thus ?case
-   by(auto simp: pref_match_def P\<^sub>a_set card_distinct match_def index_nth_id prefers_def opti\<^sub>a_def \<alpha>_def cong: conj_cong)
+   by(auto simp: pref_match_def P_set card_distinct match_def index_nth_id prefers_def opti\<^sub>a_def \<alpha>_def cong: conj_cong)
 next
   case 3 thus ?case using pref_match_stable atLeast0_lessThan_Suc by force
 next
   case (2 v A B M a a' ai)
   have R': "M ! match A a \<Longrightarrow>
-    (R\<^sub>b ! match A (B ! match A a) ! a < R\<^sub>b ! match A (B ! match A a) ! (B ! match A a)) =
-     (P\<^sub>b ! match A (B ! match A a) \<turnstile> a < B ! match A a)"
+    (R ! match A (B ! match A a) ! a < R ! match A (B ! match A a) ! (B ! match A a)) =
+     (Q ! match A (B ! match A a) \<turnstile> a < B ! match A a)"
     using R_iff_P 2 assms by blast
   show ?case
     apply(simp only:mem_Collect_eq prod.case)
@@ -1875,7 +1875,7 @@ qed
 
 (* TODO: rm? *)
 lemma Gale_Shapley6_1_explicit:
-assumes "R\<^sub>b = map ranking P\<^sub>b"
+assumes "R = map ranking Q"
 shows "VARS A B M a a' ai b r
  [ai = 0 \<and> a = 0 \<and> A = replicate n 0 \<and> length B = n \<and> M = replicate n False]
  WHILE ai < n
@@ -1884,7 +1884,7 @@ shows "VARS A B M a a' ai b r
  DO b := match A a;
   IF \<not> M ! b
   THEN B[b] := a; M[b] := True; ai := ai + 1; a := ai
-  ELSE a' := B ! b; r := R\<^sub>b ! match A a';
+  ELSE a' := B ! b; r := R ! match A a';
        IF r ! a < r ! a'
        THEN B[b] := a; A[a'] := A!a'+1; a := a'
        ELSE A[a] := A!a+1
@@ -1894,7 +1894,7 @@ shows "VARS A B M a a' ai b r
  [matching A {<n} \<and> stable A {<n} \<and> opti\<^sub>a A]"
 proof (vcg_tc, goal_cases)
   case 1 thus ?case
-   by(auto simp: pref_match_def P\<^sub>a_set card_distinct match_def index_nth_id prefers_def opti\<^sub>a_def \<alpha>_def cong: conj_cong)
+   by(auto simp: pref_match_def P_set card_distinct match_def index_nth_id prefers_def opti\<^sub>a_def \<alpha>_def cong: conj_cong)
 next
   case 3 thus ?case using pref_match_stable atLeast0_lessThan_Suc by force
 next
@@ -1945,7 +1945,7 @@ next
         have invAB': "invAB (A[B ! match A a := A ! ?a + 1]) (\<alpha> (B[match A a := a]) M) ({<ai + 1} - {?a})"
           using invAB_swap[OF invAB[THEN conjunct1] a a' inj_dom] * match_less_n[OF A] a matched invAB
           by(simp add:\<alpha>update2)
-        have pref: "P\<^sub>b ! match A ?a \<turnstile> a < ?a" using A P\<^sub>b_set \<open>?a < n\<close> \<open>?pref\<close> a assms length_P\<^sub>b
+        have pref: "Q ! match A ?a \<turnstile> a < ?a" using A Q_set \<open>?a < n\<close> \<open>?pref\<close> a assms length_Q
           by(auto simp: match_less_n ranking_iff_pref)
         case 1 show ?case (* changed *)
           using invAM_swap[OF invAM a a' pref] invAB invAB' a' as unfolding *
@@ -1962,8 +1962,8 @@ next
         case 1
         have "invAB2 (A[a := A ! a + 1]) B M ?M" using invAB a
           by (metis match_def nth_list_update_neq ranI)
-        thus ?case using invAM_next[OF invAM a a'] \<open>\<not> ?pref\<close>  \<open>B ! match A a < n\<close> P\<^sub>b_set 2 assms
-          by (simp add: invar2'_def length_P\<^sub>b match_less_n ranking_iff_pref) (* changed *)
+        thus ?case using invAM_next[OF invAM a a'] \<open>\<not> ?pref\<close>  \<open>B ! match A a < n\<close> Q_set 2 assms
+          by (simp add: invar2'_def length_Q match_less_n ranking_iff_pref) (* changed *)
         case 2
         show ?case using a v var_next[OF m M _ pref_match1, of a]
           by (metis Suc_eq_plus1 atLeast0LessThan lessThan_iff) 
@@ -1978,33 +1978,33 @@ end
 subsection \<open>Functional implementation\<close>
 
 definition
-"gs_inner P\<^sub>a R\<^sub>b M =
+"gs_inner P R M =
   while (\<lambda>(A,B,a,b). M!b)
     (\<lambda>(A,B,a,b).
       let a' = B ! b;
-          r = R\<^sub>b ! (P\<^sub>a ! a' ! (A ! a')) in
+          r = R ! (P ! a' ! (A ! a')) in
       let (A, B, a) =
         if r ! a < r ! a'
         then (A[a' := A!a' + 1], B[b := a], a')
         else (A[a := A!a + 1], B, a)
-      in (A, B, a, P\<^sub>a ! a ! (A ! a)))"
+      in (A, B, a, P ! a ! (A ! a)))"
 
 definition
-"gs n P\<^sub>a R\<^sub>b =
+"gs n P R =
   while (\<lambda>(A,B,M,ai). ai < n)
    (\<lambda>(A,B,M,ai).
-     let (A,B,a,b) = gs_inner P\<^sub>a R\<^sub>b M (A, B, ai, P\<^sub>a ! ai ! (A ! ai))
+     let (A,B,a,b) = gs_inner P R M (A, B, ai, P ! ai ! (A ! ai))
      in (A, B[b:=a], M[b:=True], ai+1))
   (replicate n 0, replicate n 0, replicate n False,0)"
 
 definition
-"gs1 n P\<^sub>a R\<^sub>b =
+"gs1 n P R =
   while (\<lambda>(A,B,M,ai,a). ai < n)
    (\<lambda>(A,B,M,ai,a).
-     let b = P\<^sub>a ! a ! (A ! a) in
+     let b = P ! a ! (A ! a) in
      if \<not> M ! b
      then (A, B[b := a], M[b := True], ai+1, ai+1)
-     else let a' = B ! b; r = R\<^sub>b ! (P\<^sub>a ! a' ! (A ! a')) in
+     else let a' = B ! b; r = R ! (P ! a' ! (A ! a')) in
        if r ! a < r ! a'
        then (A[a' := A!a'+1], B[b := a], M, ai, a')
        else (A[a := A!a+1], B, M, ai, a))
@@ -2014,20 +2014,20 @@ context Pref
 begin
 
 lemma gs_inner:
-assumes "R\<^sub>b = map ranking P\<^sub>b"
+assumes "R = map ranking Q"
 assumes "invar2 A B M ai a" "b = match A a"
-shows "gs_inner P\<^sub>a R\<^sub>b M (A, B, a, b) = (A',B',a',b') \<longrightarrow> invar1 A' (B'[b' := a']) (M[b' := True]) (ai+1)"
+shows "gs_inner P R M (A, B, a, b) = (A',B',a',b') \<longrightarrow> invar1 A' (B'[b' := a']) (M[b' := True]) (ai+1)"
 unfolding gs_inner_def
 proof(rule while_rule2[where P = "\<lambda>(A,B,a,b). invar2 A B M ai a \<and> b = match A a"
- and r = "measure (%(A, B, a, b). Pref.var P\<^sub>a A {<ai})"], goal_cases)
+ and r = "measure (%(A, B, a, b). Pref.var P A {<ai})"], goal_cases)
   case 1
   show ?case using assms unfolding var_def by simp
 next
   case inv: (2 s)
   obtain A B a b where s: "s =  (A, B, a, b)"
     using prod_cases4 by blast
-  have R: "\<forall>b<n. \<forall>a1<n. \<forall>a2<n. R\<^sub>b ! b ! a1 < R\<^sub>b ! b ! a2 \<longleftrightarrow> P\<^sub>b ! b \<turnstile> a1 < a2"
-    by (simp add: P\<^sub>b_set \<open>R\<^sub>b = _\<close> length_P\<^sub>b ranking_iff_pref)
+  have R: "\<forall>b<n. \<forall>a1<n. \<forall>a2<n. R ! b ! a1 < R ! b ! a2 \<longleftrightarrow> Q ! b \<turnstile> a1 < a2"
+    by (simp add: Q_set \<open>R = _\<close> length_Q ranking_iff_pref)
   show ?case
   proof(rule, goal_cases)
     case 1 show ?case
@@ -2050,20 +2050,20 @@ next
   show ?case by simp
 qed
 
-lemma gs: assumes "R\<^sub>b = map ranking P\<^sub>b"
-shows "gs n P\<^sub>a R\<^sub>b = (A,BMai) \<longrightarrow> matching A {<n} \<and> stable A {<n} \<and> opti\<^sub>a A"
+lemma gs: assumes "R = map ranking Q"
+shows "gs n P R = (A,BMai) \<longrightarrow> matching A {<n} \<and> stable A {<n} \<and> opti\<^sub>a A"
 unfolding gs_def
 proof(rule while_rule2[where P = "\<lambda>(A,B,M,ai). invar1 A B M ai"
   and r = "measure(\<lambda>(A,B,M,ai). n - ai)"], goal_cases)
   case 1 show ?case
-   by(auto simp: stable_def pref_match_def P\<^sub>a_set card_distinct match_def index_nth_id prefers_def opti\<^sub>a_def \<alpha>_def cong: conj_cong)
+   by(auto simp: stable_def pref_match_def P_set card_distinct match_def index_nth_id prefers_def opti\<^sub>a_def \<alpha>_def cong: conj_cong)
 next
   case (2 s)
   obtain A B M ai where s: "s =  (A, B, M, ai)"
     using prod_cases4 by blast
   have 1: "invar2 A B M ai ai" using 2 s
     by (auto simp: atLeastLessThanSuc_atLeastAtMost simp flip: atLeastLessThan_eq_atLeastAtMost_diff)
-  show ?case using 2 s gs_inner[OF \<open>R\<^sub>b = _ \<close> 1] by (auto simp: match_def simp del: invar1_def split: prod.split)
+  show ?case using 2 s gs_inner[OF \<open>R = _ \<close> 1] by (auto simp: match_def simp del: invar1_def split: prod.split)
 next
   case 3
   thus ?case using pref_match_stable by auto
@@ -2073,21 +2073,21 @@ next
 qed
 
 
-lemma gs1: assumes "R\<^sub>b = map ranking P\<^sub>b"
-shows "gs1 n P\<^sub>a R\<^sub>b = (A,BMaia) \<longrightarrow> matching A {<n} \<and> stable A {<n} \<and> opti\<^sub>a A"
+lemma gs1: assumes "R = map ranking Q"
+shows "gs1 n P R = (A,BMaia) \<longrightarrow> matching A {<n} \<and> stable A {<n} \<and> opti\<^sub>a A"
 unfolding gs1_def
 proof(rule while_rule2[where P = "\<lambda>(A,B,M,ai,a). invar2' A B M ai a"
-  and r = "measure (%(A, B, M, ai, a). Pref.var P\<^sub>a A ({<ai+1} - {a}))"], goal_cases)
+  and r = "measure (%(A, B, M, ai, a). Pref.var P A ({<ai+1} - {a}))"], goal_cases)
   case 1 show ?case
-    by(auto simp: stable_def pref_match_def P\<^sub>a_set card_distinct match_def index_nth_id prefers_def opti\<^sub>a_def \<alpha>_def cong: conj_cong)
+    by(auto simp: stable_def pref_match_def P_set card_distinct match_def index_nth_id prefers_def opti\<^sub>a_def \<alpha>_def cong: conj_cong)
 next
   case (2 s)
   obtain A B M ai a where s: "s =  (A, B, M, ai, a)"
     using prod_cases5 by blast
   hence 1: "invar2' A B M ai a" "ai < n" using 2 by (simp_all)
   have R': "M ! match A a \<Longrightarrow>
-    (R\<^sub>b ! match A (B ! match A a) ! a < R\<^sub>b ! match A (B ! match A a) ! (B ! match A a)) =
-     (P\<^sub>b ! match A (B ! match A a) \<turnstile> a < B ! match A a)"
+    (R ! match A (B ! match A a) ! a < R ! match A (B ! match A a) ! (B ! match A a)) =
+     (Q ! match A (B ! match A a) \<turnstile> a < B ! match A a)"
     using R_iff_P[OF assms 1] by linarith
   show ?case 
     using 1 R' pres2'[OF 1]
@@ -2111,22 +2111,22 @@ end
 subsection \<open>Executable functional Code\<close>
 
 definition
-"Gale_Shapley P\<^sub>a P\<^sub>b = (if Pref P\<^sub>a P\<^sub>b then Some (fst (gs (length P\<^sub>a) P\<^sub>a (map ranking P\<^sub>b))) else None)"
+"Gale_Shapley P Q = (if Pref P Q then Some (fst (gs (length P) P (map ranking Q))) else None)"
 
-theorem gs: "\<lbrakk> Pref P\<^sub>a P\<^sub>b; n = length P\<^sub>a \<rbrakk> \<Longrightarrow>
- \<exists>A. Gale_Shapley P\<^sub>a P\<^sub>b = Some(A) \<and> Pref.matching P\<^sub>a A {<n} \<and>
-   Pref.stable P\<^sub>a P\<^sub>b A {<n} \<and> Pref.opti\<^sub>a P\<^sub>a P\<^sub>b A"
+theorem gs: "\<lbrakk> Pref P Q; n = length P \<rbrakk> \<Longrightarrow>
+ \<exists>A. Gale_Shapley P Q = Some(A) \<and> Pref.matching P A {<n} \<and>
+   Pref.stable P Q A {<n} \<and> Pref.opti\<^sub>a P Q A"
 unfolding Gale_Shapley_def using Pref.gs
 by (metis fst_conv surj_pair)
 
 declare Pref_def [code]
 
 definition
-"Gale_Shapley1 P\<^sub>a P\<^sub>b = (if Pref P\<^sub>a P\<^sub>b then Some (fst (gs1 (length P\<^sub>a) P\<^sub>a (map ranking P\<^sub>b))) else None)"
+"Gale_Shapley1 P Q = (if Pref P Q then Some (fst (gs1 (length P) P (map ranking Q))) else None)"
 
-theorem gs1: "\<lbrakk> Pref P\<^sub>a P\<^sub>b; n = length P\<^sub>a \<rbrakk> \<Longrightarrow>
- \<exists>A. Gale_Shapley1 P\<^sub>a P\<^sub>b = Some(A) \<and> Pref.matching P\<^sub>a A {<n} \<and>
-   Pref.stable P\<^sub>a P\<^sub>b A {<n} \<and> Pref.opti\<^sub>a P\<^sub>a P\<^sub>b A"
+theorem gs1: "\<lbrakk> Pref P Q; n = length P \<rbrakk> \<Longrightarrow>
+ \<exists>A. Gale_Shapley1 P Q = Some(A) \<and> Pref.matching P A {<n} \<and>
+   Pref.stable P Q A {<n} \<and> Pref.opti\<^sub>a P Q A"
 unfolding Gale_Shapley1_def using Pref.gs1
 by (metis fst_conv surj_pair)
 
