thys/Gale_Shapley/Gale_Shapley2.thy
@@ -29,7 +29,7 @@ begin
 
 subsection \<open>Algorithm 7: Arrays\<close>
 
-definition "match_array A a = P\<^sub>a ! a ! (A !! a)"
+definition "match_array A a = P ! a ! (A !! a)"
 
 lemma match_array: "match_array A a = match (list A) a"
 by(cases A) (simp add: match_array_def match_def)
@@ -37,7 +37,7 @@ by(cases A) (simp add: match_array_def match_def)
 lemmas array_abs = match_array array_list_of_set array_get
 
 lemma Gale_Shapley7:
-assumes "R = map ranking P\<^sub>b"
+assumes "R = map ranking Q"
 shows
 "VARS A B M ai a a' b r
  [ai = 0 \<and> A = array 0 n \<and> B = array 0 n \<and> M = array False n]
@@ -60,14 +60,14 @@ shows
  [matching (list A) {<n} \<and> stable (list A) {<n} \<and> opti\<^sub>a (list A)]"
 proof (vcg_tc, goal_cases)
   case 1 thus ?case  (* outer invar holds initially *)
-   by(auto simp:  pref_match_def P\<^sub>a_set card_distinct match_def list_array index_nth_id prefers_def opti\<^sub>a_def \<alpha>_def cong: conj_cong)
+   by(auto simp:  pref_match_def P_set card_distinct match_def list_array index_nth_id prefers_def opti\<^sub>a_def \<alpha>_def cong: conj_cong)
 next
   case 2 (* outer invar and b implies inner invar *)
   thus ?case by (auto simp: atLeastLessThanSuc_atLeastAtMost simp flip: atLeastLessThan_eq_atLeastAtMost_diff)
 next
   case 3 (* preservation of inner invar *)
-  have R: "\<forall>b<n. \<forall>a1<n. \<forall>a2<n. R ! b ! a1 < R ! b ! a2 \<longleftrightarrow> P\<^sub>b ! b \<turnstile> a1 < a2"
-    by (simp add: P\<^sub>b_set \<open>R = _\<close> length_P\<^sub>b ranking_iff_pref)
+  have R: "\<forall>b<n. \<forall>a1<n. \<forall>a2<n. R ! b ! a1 < R ! b ! a2 \<longleftrightarrow> Q ! b \<turnstile> a1 < a2"
+    by (simp add: Q_set \<open>R = _\<close> length_Q ranking_iff_pref)
   show ?case
   proof (simp only: mem_Collect_eq prod.case, goal_cases)
     case 1 show ?case using inner_pres[OF R _ _ refl refl refl] 3
@@ -90,7 +90,7 @@ qed
 subsection \<open>Algorithm 7.1: single-loop variant\<close>
 
 lemma Gale_Shapley7_1:
-assumes "R\<^sub>b = map ranking P\<^sub>b"
+assumes "R = map ranking Q"
 shows "VARS A B M a a' ai b r
  [ai = 0 \<and> a = 0 \<and> A = array 0 n \<and> B = array 0 n \<and> M = array False n]
  WHILE ai < n
@@ -99,7 +99,7 @@ shows "VARS A B M a a' ai b r
  DO b := match_array A a;
   IF \<not> M !! b
   THEN B := B[b ::= a]; M := M[b ::= True]; ai := ai + 1; a := ai
-  ELSE a' := B !! b; r := R\<^sub>b ! match_array A a';
+  ELSE a' := B !! b; r := R ! match_array A a';
        IF r ! a < r ! a'
        THEN B := B[b ::= a]; A := A[a' ::= A!!a' + 1]; a := a'
        ELSE A := A[a ::= A!!a + 1]
@@ -109,14 +109,14 @@ shows "VARS A B M a a' ai b r
  [matching (list A) {<n} \<and> stable (list A) {<n} \<and> opti\<^sub>a (list A)]"
 proof (vcg_tc, goal_cases)
   case 1 thus ?case
-   by(auto simp:  pref_match_def P\<^sub>a_set card_distinct match_def list_array index_nth_id prefers_def opti\<^sub>a_def \<alpha>_def cong: conj_cong)
+   by(auto simp:  pref_match_def P_set card_distinct match_def list_array index_nth_id prefers_def opti\<^sub>a_def \<alpha>_def cong: conj_cong)
 next
   case 3 thus ?case using pref_match_stable atLeast0_lessThan_Suc[of n] by force
 next
   case (2 v A B M a a' ai)
   have R': "M !! match_array A a \<Longrightarrow>
-    (R\<^sub>b ! match_array A (B !! match_array A a) ! a < R\<^sub>b ! match_array A (B !! match_array A a) ! (B !! match_array A a)) =
-     (P\<^sub>b ! match_array A (B !! match_array A a) \<turnstile> a < B !! match_array A a)"
+    (R ! match_array A (B !! match_array A a) ! a < R ! match_array A (B !! match_array A a) ! (B !! match_array A a)) =
+     (Q ! match_array A (B !! match_array A a) \<turnstile> a < B !! match_array A a)"
     using R_iff_P 2 assms by (metis array_abs)
   show ?case
     apply(simp only:mem_Collect_eq prod.case)
@@ -129,37 +129,37 @@ end
 subsection \<open>Executable functional Code\<close>
 
 definition gs_inner where
-"gs_inner P\<^sub>a R M =
+"gs_inner P R M =
   while (\<lambda>(A,B,a,b). M !! b)
     (\<lambda>(A,B,a,b).
       let a' = B !! b;
-          r = R !! (P\<^sub>a !! a' !! (A !! a')) in
+          r = R !! (P !! a' !! (A !! a')) in
       let (A, B, a) =
         if r !! a < r !! a'
         then (A[a' ::= A !! a' + 1], B[b ::= a], a')
         else (A[a ::= A !! a + 1], B, a)
-      in (A, B, a, P\<^sub>a !! a !! (A !! a)))"
+      in (A, B, a, P !! a !! (A !! a)))"
 
 definition gs :: "nat \<Rightarrow> nat array array \<Rightarrow> nat array array
   \<Rightarrow> nat array \<times> nat array \<times> bool array \<times> nat" where
-"gs n P\<^sub>a R =
+"gs n P R =
   while (\<lambda>(A,B,M,ai). ai < n)
    (\<lambda>(A,B,M,ai).
-     let (A,B,a,b) = gs_inner P\<^sub>a R M (A, B, ai, P\<^sub>a !! ai !! (A !! ai))
+     let (A,B,a,b) = gs_inner P R M (A, B, ai, P !! ai !! (A !! ai))
      in (A, B[b ::= a], M[b::=True], ai+1))
   (array 0 n, array 0 n, array False n, 0)"
 
 
 definition gs1 :: "nat \<Rightarrow> nat array array \<Rightarrow> nat array array
   \<Rightarrow> nat array \<times> nat array \<times> bool array \<times> nat \<times> nat"  where
-"gs1 n P\<^sub>a R =
+"gs1 n P R =
   while (\<lambda>(A,B,M,ai,a). ai < n)
    (\<lambda>(A,B,M,ai,a).
-     let b = P\<^sub>a !! a !! (A !! a)
+     let b = P !! a !! (A !! a)
      in if \<not> M !! b
         then (A, B[b ::= a], M[b ::= True], ai+1, ai+1)
         else let a' = B !! b;
-                 r = R !! (P\<^sub>a !! a' !! (A !! a'))
+                 r = R !! (P !! a' !! (A !! a'))
              in if r !!  a < r !! a'
                 then (A[a' ::= A!!a' + 1], B[b ::= a], M, ai, a')
                 else (A[a ::= A!!a + 1], B, M, ai, a))
@@ -194,15 +194,15 @@ lemma rank_array1_iff_pref:  "\<lbrakk> set P = {<length P}; i < length P; j < l
 by(simp add: rank_array1_def prefers_def nth_rk_of_pref card_distinct)
 
 definition Gale_Shapley where
-"Gale_Shapley P\<^sub>a P\<^sub>b =
-  (if Pref P\<^sub>a P\<^sub>b
-   then Some (fst (gs (length P\<^sub>a) (pref_array P\<^sub>a) (rank_array P\<^sub>b)))
+"Gale_Shapley P Q =
+  (if Pref P Q
+   then Some (fst (gs (length P) (pref_array P) (rank_array Q)))
    else None)"
 
 definition Gale_Shapley1 where
-"Gale_Shapley1 P\<^sub>a P\<^sub>b =
-  (if Pref P\<^sub>a P\<^sub>b
-   then Some (fst (gs1 (length P\<^sub>a) (pref_array P\<^sub>a) (rank_array P\<^sub>b)))
+"Gale_Shapley1 P Q =
+  (if Pref P Q
+   then Some (fst (gs1 (length P) (pref_array P) (rank_array Q)))
    else None)"
 
 (*export_code Gale_Shapley_array in SML*)
@@ -211,14 +211,14 @@ context Pref
 begin
 
 lemma gs_inner:
-assumes "R = rank_array P\<^sub>b"
+assumes "R = rank_array Q"
 assumes "invar2 (list A) (list B) (list M) ai a" "b = match_array A a"
-shows "gs_inner (pref_array P\<^sub>a) R M (A, B, a, b) = (A',B',a',b')
+shows "gs_inner (pref_array P) R M (A, B, a, b) = (A',B',a',b')
   \<longrightarrow> invar1 (list A') ((list B')[b' := a']) ((list M)[b' := True]) (ai+1)"
 unfolding gs_inner_def
 proof(rule while_rule2[where
      P = "\<lambda>(A,B,a,b). invar2 (list A) (list B) (list M) ai a \<and> b = match_array A a"
- and r = "measure (\<lambda>(A, B, a, b). Pref.var0 P\<^sub>a (list A) {<n})"], goal_cases)
+ and r = "measure (\<lambda>(A, B, a, b). Pref.var0 P (list A) {<n})"], goal_cases)
   case 1
   show ?case using assms unfolding var_def by simp
 next
@@ -232,13 +232,13 @@ next
     hence 2: "list A ! a < n" using s inv(1)[unfolded invar2_def]
       apply simp using "*" wf_less_n by presburger
     hence "match (list A) a < n"
-      by (metis "*" P\<^sub>a_set atLeast0LessThan lessThan_iff match_def nth_mem)
+      by (metis "*" P_set atLeast0LessThan lessThan_iff match_def nth_mem)
     from this have **: "list B ! match (list A) a < n" using s inv[unfolded invar2_def]
       apply (simp add: array_abs ran_def) using atLeast0LessThan by blast
-    have R: "\<forall>b<n. \<forall>a1<n. \<forall>a2<n. map list (list R) ! b ! a1 < map list (list R) ! b ! a2 \<longleftrightarrow> P\<^sub>b ! b \<turnstile> a1 < a2"
-    using rank_array1_iff_pref by(simp add: \<open>R = _\<close> length_P\<^sub>b array_get P\<^sub>b_set rank_array_def)
+    have R: "\<forall>b<n. \<forall>a1<n. \<forall>a2<n. map list (list R) ! b ! a1 < map list (list R) ! b ! a2 \<longleftrightarrow> Q ! b \<turnstile> a1 < a2"
+    using rank_array1_iff_pref by(simp add: \<open>R = _\<close> length_Q array_get Q_set rank_array_def)
     have ***: "match (list A) (list B ! b) < length (list R)"  using s inv(1)[unfolded invar2_def]
-      using ** by(simp add: \<open>R = _\<close> rank_array_def match_array match_less_n length_P\<^sub>b)
+      using ** by(simp add: \<open>R = _\<close> rank_array_def match_array match_less_n length_Q)
     show ?case
     using inv apply(simp only: s prod.case Let_def split: if_split)
     using inner_pres[OF R _ _ refl refl refl refl refl, of "list A" "list B" "list M" ai a b]
@@ -263,13 +263,13 @@ next
   show ?case by simp
 qed
 
-lemma gs: assumes "R = rank_array P\<^sub>b"
-shows "gs n (pref_array P\<^sub>a) R = (A,B,M,ai) \<longrightarrow> matching (list A) {<n} \<and> stable (list A) {<n} \<and> opti\<^sub>a (list A)"
+lemma gs: assumes "R = rank_array Q"
+shows "gs n (pref_array P) R = (A,B,M,ai) \<longrightarrow> matching (list A) {<n} \<and> stable (list A) {<n} \<and> opti\<^sub>a (list A)"
 unfolding gs_def
 proof(rule while_rule2[where P = "\<lambda>(A,B,M,ai). invar1 (list A) (list B) (list M) ai"
   and r = "measure(\<lambda>(A,B,M,ai). n - ai)"], goal_cases)
   case 1 show ?case
-   by(auto simp: pref_match_def P\<^sub>a_set card_distinct match_def list_array index_nth_id prefers_def opti\<^sub>a_def \<alpha>_def cong: conj_cong)
+   by(auto simp: pref_match_def P_set card_distinct match_def list_array index_nth_id prefers_def opti\<^sub>a_def \<alpha>_def cong: conj_cong)
 next
   case (2 s)
   obtain A B M ai where s: "s =  (A, B, M, ai)"
@@ -290,13 +290,13 @@ qed
 
 
 lemma R_iff_P:
-assumes "R\<^sub>b = rank_array P\<^sub>b" "invar2' A B M ai a" "ai < n" "M ! match A a"
+assumes "R = rank_array Q" "invar2' A B M ai a" "ai < n" "M ! match A a"
   "b = match A a" "a' = B ! b"
-shows "(list (list R\<^sub>b ! match A a') ! a < list (list R\<^sub>b ! match A a') ! a')
-       = (P\<^sub>b ! match A a' \<turnstile> a < a')"
+shows "(list (list R ! match A a') ! a < list (list R ! match A a') ! a')
+       = (Q ! match A a' \<turnstile> a < a')"
 proof -
-  have R: "\<forall>b<n. \<forall>a1<n. \<forall>a2<n. R\<^sub>b !! b !! a1 < R\<^sub>b !! b !! a2 \<longleftrightarrow> P\<^sub>b ! b \<turnstile> a1 < a2"
-    by (simp add: P\<^sub>b_set \<open>R\<^sub>b = _\<close> length_P\<^sub>b array_of_list_def rank_array_def rank_array1_iff_pref)
+  have R: "\<forall>b<n. \<forall>a1<n. \<forall>a2<n. R !! b !! a1 < R !! b !! a2 \<longleftrightarrow> Q ! b \<turnstile> a1 < a2"
+    by (simp add: Q_set \<open>R = _\<close> length_Q array_of_list_def rank_array_def rank_array1_iff_pref)
   let ?M = "{<ai+1} - {a}"
   have A: "wf A" and M: "?M \<subseteq> {<n}" and as: "a < n" and invAB: "invAB2 A B M ?M"
       using assms(2,3) by auto
@@ -307,13 +307,13 @@ proof -
 qed
 
 
-lemma gs1: assumes "R\<^sub>b = rank_array P\<^sub>b"
-shows "gs1 n (pref_array P\<^sub>a) R\<^sub>b = (A,B,M,ai,a) \<longrightarrow> matching (list A) {<n} \<and> stable (list A) {<n} \<and> opti\<^sub>a (list A)"
+lemma gs1: assumes "R = rank_array Q"
+shows "gs1 n (pref_array P) R = (A,B,M,ai,a) \<longrightarrow> matching (list A) {<n} \<and> stable (list A) {<n} \<and> opti\<^sub>a (list A)"
 unfolding gs1_def
 proof(rule while_rule2[where P = "\<lambda>(A,B,M,ai,a). invar2' (list A) (list B) (list M) ai a"
-  and r = "measure(\<lambda>(A,B,M,ai,a). Pref.var P\<^sub>a (list A) ({<ai+1} - {a}))"], goal_cases)
+  and r = "measure(\<lambda>(A,B,M,ai,a). Pref.var P (list A) ({<ai+1} - {a}))"], goal_cases)
   case 1 show ?case
-   by(auto simp: pref_match_def P\<^sub>a_set card_distinct match_def list_array index_nth_id prefers_def opti\<^sub>a_def \<alpha>_def cong: conj_cong)
+   by(auto simp: pref_match_def P_set card_distinct match_def list_array index_nth_id prefers_def opti\<^sub>a_def \<alpha>_def cong: conj_cong)
 next
   case (2 s)
   obtain A B M ai a where s: "s =  (A, B, M, ai, a)"
@@ -327,10 +327,10 @@ next
     using s 1[unfolded invar2'_def] apply (simp add: array_abs ran_def)
     using atLeast0LessThan by blast
   have R': "list M ! match (list A) a \<Longrightarrow>
-    (list (list R\<^sub>b ! match (list A) (list B ! match (list A) a)) ! a
-     < list (list R\<^sub>b ! match (list A) (list B ! match (list A) a)) ! (list B ! match (list A) a)) =
-     (P\<^sub>b ! match (list A) (list B ! match (list A) a) \<turnstile> a < list B ! match (list A) a)"
-    using R_iff_P \<open>R\<^sub>b = _\<close> 1 \<open>ai < n\<close> by blast
+    (list (list R ! match (list A) (list B ! match (list A) a)) ! a
+     < list (list R ! match (list A) (list B ! match (list A) a)) ! (list B ! match (list A) a)) =
+     (Q ! match (list A) (list B ! match (list A) a) \<turnstile> a < list B ! match (list A) a)"
+    using R_iff_P \<open>R = _\<close> 1 \<open>ai < n\<close> by blast
   show ?case
     using s apply (simp add: Let_def)
     unfolding list_list_pref_array[OF \<open>a < n\<close>[unfolded n_def]] array_abs
@@ -346,15 +346,15 @@ qed
 
 end
 
-theorem gs: "\<lbrakk> Pref P\<^sub>a P\<^sub>b; n = length P\<^sub>a \<rbrakk> \<Longrightarrow>
- \<exists>A. Gale_Shapley P\<^sub>a P\<^sub>b = Some A
-   \<and> Pref.matching P\<^sub>a (list A) {<n} \<and> Pref.stable P\<^sub>a P\<^sub>b (list A) {<n} \<and> Pref.opti\<^sub>a P\<^sub>a P\<^sub>b (list A)"
+theorem gs: "\<lbrakk> Pref P Q; n = length P \<rbrakk> \<Longrightarrow>
+ \<exists>A. Gale_Shapley P Q = Some A
+   \<and> Pref.matching P (list A) {<n} \<and> Pref.stable P Q (list A) {<n} \<and> Pref.opti\<^sub>a P Q (list A)"
 unfolding Gale_Shapley_def using Pref.gs
 by (metis fst_conv surj_pair)
 
-theorem gs1: "\<lbrakk> Pref P\<^sub>a P\<^sub>b; n = length P\<^sub>a \<rbrakk> \<Longrightarrow>
- \<exists>A. Gale_Shapley1 P\<^sub>a P\<^sub>b = Some A
-   \<and> Pref.matching P\<^sub>a (list A) {<n} \<and> Pref.stable P\<^sub>a P\<^sub>b (list A) {<n} \<and> Pref.opti\<^sub>a P\<^sub>a P\<^sub>b (list A)"
+theorem gs1: "\<lbrakk> Pref P Q; n = length P \<rbrakk> \<Longrightarrow>
+ \<exists>A. Gale_Shapley1 P Q = Some A
+   \<and> Pref.matching P (list A) {<n} \<and> Pref.stable P Q (list A) {<n} \<and> Pref.opti\<^sub>a P Q (list A)"
 unfolding Gale_Shapley1_def using Pref.gs1
 by (metis fst_conv surj_pair)
 
